Annotated.v
@@ -9,7 +9,7 @@ Import BigStep.BigStep.Dom.Prog.
 Record sign : Set := make_sign {
   lvt : Var -> L.t';
   resType : option L.t';
-  resExceptionType : ClassName -> L.t;
+  (* DEX resExceptionType : ClassName -> L.t;*)
   heapEffect : L.t
 }.
 
@@ -17,7 +17,7 @@ Definition default_signature : sign :=
   make_sign
     (fun _ => L.Simple L.bot)
     None
-    (fun _ => L.bot)
+    (* DEX (fun _ => L.bot) *)
     L.bot.    
 
 
@@ -26,10 +26,13 @@ Record ExtendedProgram : Type := extP {
   newArT : Method * PC -> L.t';
   static_signature : ShortMethodSignature -> sign;
   virtual_signature : ShortMethodSignature -> L.t -> sign;
-  ft : FieldSignature -> L.t'
+  ft : FieldSignature -> L.t';
+  locR : ShortMethodSignature -> list Var
 }.
 
+(* DEX
 Definition throwableBy (p:Program) := PROG.throwableBy p.
+*)
 
 (*
 Definition static_signature (p:ExtendedProgram) mid : sign :=
@@ -42,32 +45,41 @@ Definition  virtual_signature (p:ExtendedProgram) mid (k:L.t) : sign :=
   static_signature p mid.
 *)
 
+(* DEX
 Definition well_formed_lookupswitch m := forall pc def l i o1 o2,
   instructionAt m pc = Some (Lookupswitch def l) ->
   In (i, o1) l -> In (i, o2) l -> o1=o2.
+*)
 
+(* DEX
 Definition np := (javaLang,NullPointerException).
 Definition cc := (javaLang,ClassCastException).
 Definition ae := (javaLang,ArithmeticException).
 Definition nase := (javaLang,NegativeArraySizeException).
 Definition iob := (javaLang,ArrayIndexOutOfBoundsException).
 Definition ase := (javaLang,ArrayStoreException).
+*)
 
 Definition tag := option ClassName.
 
+(* DEX
 Definition TypeStack := list L.t'.
+*)
+Module VarMap := BinNatMap.
+Definition TypeRegisters := VarMap.t L.t'.
 
+(* DEX
 Definition compat_type_st_lvt (s:sign) (st:TypeStack) (n:nat) : Prop :=
   forall x, ((Var_toN x)<n)%nat -> exists k,
     nth_error st (n-(Var_toN x)-1)%nat = Some k /\
     L.leql' k (lvt s x).
+*)
 
+(* DEX
 Definition elift m pc k st :=
   match throwableAt m pc with
     | nil => st
     | _ => lift k st
   end.
-
-
-
+*)
 
