ImplemDomain.v
@@ -1,0 +1,1600 @@
+(** * Bicolano: Semantic domains (interface implementation) *)
+
+Require Export ImplemProgramWithMap.
+Require Export Domain.
+
+ 
+Ltac caseeq t := generalize (refl_equal t); pattern t at -1 in |- * ; case t.
+
+(** All semantic domains and basic operation are encapsulated in a module signature *)
+
+Module Dom <: SEMANTIC_DOMAIN.
+
+ (** We depend on the choices done for program data structures *)
+ Module Prog := ImplemProgramWithMap.Make.
+ Import Prog.
+
+Open Scope Z_scope.
+ Module SByte <: Numeric.NUMSIZE. Definition power := 7%nat. End SByte.
+ Module SShort<: Numeric.NUMSIZE. Definition power := 15%nat. End SShort.
+ Module SInt  <: Numeric.NUMSIZE. Definition power := 31%nat. End SInt.
+
+ Module Byte  : Numeric.NUMERIC with Definition power := 7%nat := Numeric.Make SByte.
+ Module Short : Numeric.NUMERIC with Definition power := 15%nat := Numeric.Make SShort.
+ Module Int   : Numeric.NUMERIC with Definition power := 31%nat := Numeric.Make SInt.
+
+ (** conversion *)
+ Definition b2i (b:Byte.t) : Int.t := Int.const (Byte.toZ b).
+ Definition s2i (s:Short.t) : Int.t := Int.const (Short.toZ s).
+ Definition i2b (i:Int.t) : Byte.t := Byte.const (Int.toZ i).
+ Definition i2s (i:Int.t) : Short.t := Short.const (Int.toZ i).
+ Definition i2bool (i:Int.t) : Byte.t := Byte.const (Int.toZ i mod 2).
+
+ Inductive num : Set :=
+   | I : Int.t -> num
+   | B : Byte.t -> num
+   | Sh : Short.t -> num.
+ 
+ (** Location is the domain of adresses in the heap *)
+ Definition Location : Set := N.
+ Definition Location_dec : forall loc1 loc2:Location,{loc1=loc2}+{~loc1=loc2} :=
+   (Aeq_Dec _ _ Neq_spec).
+
+ Inductive value : Set :=
+   | Num : num -> value
+   | Ref: Location -> value
+   | Null : value.
+
+ Definition init_value (t:type) : value :=
+    match t with
+     | ReferenceType _ => Null
+     | PrimitiveType _ => Num (I (Int.const 0))
+    end.
+
+ Definition init_field_value (f:Field) : value :=
+   match FIELD.initValue f with
+    | FIELD.Int z => Num (I (Int.const z))
+    | FIELD.NULL => Null
+    | FIELD.UNDEF => init_value (FIELDSIGNATURE.type (FIELD.signature f))
+  end.
+ 
+ (** Domain of local variables *)
+ Module Type LOCALVAR.
+   Parameter t : Type.
+   Parameter get : t-> Var -> option value.
+   Parameter update : t -> Var -> value -> t.
+   Parameter ret : Var.
+   Parameter ex : Var.
+   Parameter get_update_new : forall l x v, get (update l x v) x = Some v.
+   Parameter get_update_old : forall l x y v,
+     x<>y -> get (update l x v) y = get l y.
+ End LOCALVAR.
+
+ Module MapVar <: MAP with Definition key := Var := BinNatMap.
+
+ Module LocalVar <: LOCALVAR.
+   Definition t := MapVar.t value.
+   Definition get : t -> Var -> option value := @MapVar.get value.
+   Definition update : t -> Var -> value -> t := @MapVar.update value.
+   Definition ret := Npos (xO (xO (xO (xO (xO (xO (xO (xO 
+     (xO (xO (xO (xO (xO (xO (xO (xO xH)))))))))))))))).
+   Definition ex := Npos (xI (xO (xO (xO (xO (xO (xO (xO 
+     (xO (xO (xO (xO (xO (xO (xO (xO xH)))))))))))))))).  
+   Lemma get_update_new : forall l x v, get (update l x v) x = Some v.
+   Proof. exact (MapVar.get_update1 value). Qed.
+   Lemma get_update_old : forall l x y v,
+     x<>y -> get (update l x v) y = get l y.
+   Proof. 
+    intros;refine (MapVar.get_update2 value _ _ _ _ _). 
+    intro;apply H;subst;trivial.
+  Qed.
+  Definition empty := MapVar.empty value.
+ End LocalVar.
+
+ Fixpoint listvar2localvar_rec
+    (l_ori:LocalVar.t) (n:nat) (lv:list Var) (l:LocalVar.t) {struct n}: LocalVar.t :=
+   match n with 
+   | O => l
+   | S n =>
+     match lv with 
+     | nil => l
+     | h :: t =>
+       match LocalVar.get l_ori h with
+       | None =>
+         listvar2localvar_rec l_ori n t l
+       | Some v => 
+         listvar2localvar_rec l_ori n t (LocalVar.update l (N_toVar n) v)
+       end
+     end
+   end.
+ Definition listvar2localvar (l_ori:LocalVar.t) (n:nat) (lv:list Var)
+   := listvar2localvar_rec l_ori n lv LocalVar.empty.
+(*
+ (* Domain of operand stacks *) 
+ Module Type OPERANDSTACK.
+   Definition t : Set := list value.
+   Definition empty : t := nil.
+   Definition push : value -> t -> t := fun v t => cons v t.
+   Definition size : t -> nat := fun t  => length t .
+   Definition get_nth : t -> nat -> option value := fun s n => nth_error s n.
+ End OPERANDSTACK.
+
+ Module OperandStack <: OPERANDSTACK.
+   Definition t : Set := list value.
+   Definition empty : t := nil.
+   Definition push : value -> t -> t := fun v t => cons v t.
+   Definition size : t -> nat := fun t  => length t .
+   Definition get_nth : t -> nat -> option value := fun s n => nth_error s n.
+  End OperandStack.
+
+ (** Transfert fonction between operand stack and local variables necessary for invoke instructions *)
+  
+ Fixpoint stack2localvar_rec
+    (os:OperandStack.t) (n:nat) (l:LocalVar.t) {struct n}: LocalVar.t :=
+   match n with 
+   | O => l
+   | S n => 
+      match os with
+      | nil => l
+      | v::os => 
+         stack2localvar_rec os n (LocalVar.update l (N_toVar n) v)
+      end
+   end.
+ Definition stack2localvar os n := stack2localvar_rec os n LocalVar.empty.
+
+ Lemma stack2locvar_rec_prop1 :
+   forall n l os x, (n <= Var_toN x)%nat -> 
+     LocalVar.get (stack2localvar_rec  os n l) x = LocalVar.get l x.
+ Proof.
+  induction n;simpl;intros;trivial.
+  destruct os;simpl;intros;trivial.
+  assert (n <= Var_toN x)%nat. omega.
+  rewrite IHn;trivial.
+  unfold LocalVar.get, LocalVar.update;rewrite MapVar.get_update2;trivial.
+  intro Heq;rewrite Heq in H.
+  rewrite Var_toN_bij2 in H;omega.
+ Qed.
+
+ Lemma stack2locvar_prop1 :
+   forall s n x, (n <= Var_toN x)%nat -> LocalVar.get (stack2localvar s n) x = None.
+ Proof.
+   unfold stack2localvar;intros.
+   rewrite stack2locvar_rec_prop1;trivial.
+   exact (MapVar.get_empty _ _).
+ Qed.
+
+ Lemma stack2locvar_rec_prop2 :
+   forall n os l x, (Var_toN x < n)%nat ->
+     (forall y, (Var_toN y < n)%nat -> LocalVar.get l y = None) ->
+     LocalVar.get (stack2localvar_rec os n l) x = 
+       OperandStack.get_nth os (n-(Var_toN x)-1)%nat.
+ Proof.
+   induction n;simpl;intros.
+   elimtype False;omega.
+   destruct os.
+   rewrite H0;trivial.
+   destruct (Var_toN x);simpl;trivial.
+   destruct (n-0)%nat;trivial.
+   destruct (n-n0-1)%nat;trivial.
+   change (match Var_toN x with
+   | O => (S n)
+   | S l0 => (n - l0)
+   end - 1)%nat with (S n- Var_toN x -1)%nat.
+   assert (Var_toN x = n \/ Var_toN x < n)%nat. omega.
+   destruct H1.
+   pattern n at 2;rewrite <- H1;rewrite Var_toN_bij1.
+   rewrite stack2locvar_rec_prop1. 2:omega.
+   rewrite LocalVar.get_update_new.
+   replace (S n - Var_toN x - 1)%nat with O;try omega.
+   simpl;trivial.
+   rewrite IHn;trivial.
+   replace (S n - Var_toN x - 1)%nat with (S (n - Var_toN x - 1))%nat;try omega.
+   simpl;trivial.
+   intros;rewrite LocalVar.get_update_old.
+   apply H0;omega.
+   intro Heq;rewrite <-Heq in H2;rewrite Var_toN_bij2 in H2;omega.
+  Qed.
+   
+ Lemma stack2locvar_prop2 :
+   forall s n x, (Var_toN x < n)%nat ->
+     LocalVar.get (stack2localvar s n) x = OperandStack.get_nth s (n-(Var_toN x)-1)%nat.
+ Proof.
+  unfold stack2localvar;intros;apply stack2locvar_rec_prop2;trivial.
+  intros;exact (MapVar.get_empty _ _).
+ Qed.
+*)
+
+ Fixpoint all_super_classes (p:Program) (c:Class) (n:nat) {struct n} : option (list Class) :=
+   match n with
+     | O => None
+     | S n =>
+       match CLASS.superClass c with
+         | None => Some nil
+         | Some super_name => 
+           match PROG.class p super_name with
+             | None => None
+             | Some super => 
+               match (all_super_classes p super n) with
+                 | None => None
+                 | Some l => Some (super::l)
+               end
+           end
+       end
+   end.
+
+ Ltac inv H := inversion H; subst; clear H.
+
+ Lemma clos_refl_trans_ind2 :
+      forall (A:Type) (R:A -> A -> Prop) (P:A -> A -> Prop),
+        (forall x, P x x) ->
+        (forall x y z:A, R x y -> clos_refl_trans A R y z -> P y z  -> P x z) ->
+        forall x y, clos_refl_trans A R x y -> P x y.
+ Proof.
+   intros A R P H1 H2.
+   assert (forall x y, clos_refl_trans A R x y -> 
+              forall z, clos_refl_trans A R y z -> P y z -> P x z).
+   induction 1; eauto; intros.
+   apply IHclos_refl_trans1.
+   constructor 3 with z; auto.
+   apply IHclos_refl_trans2; auto.
+   intros.
+   apply H with y; auto.
+   constructor 2.
+ Qed.
+
+Lemma subclass_left : forall p c1 c2,
+  subclass p c1 c2 -> c1=c2 \/ (exists c, direct_subclass p c1 c /\ subclass p c c2).
+Proof.
+  intros p; unfold subclass; apply clos_refl_trans_ind2; intros; auto.
+  destruct H1; subst; auto.
+  right; exists z; auto.
+  destruct H1 as [c [T1 T2]].
+  right; exists y; split; auto.
+Qed.
+
+ Definition all_super_classes_correct : forall p n c l,
+   all_super_classes p c n = Some l ->
+   PROG.defined_Class p c -> 
+   forall c', subclass p c c' -> In c' (c::l).
+ Proof.
+   induction n; simpl.
+   intros; discriminate.
+   intros c l; case_eq (CLASS.superClass c).
+   intros c' H'.
+   case_eq (PROG.class p c'); try (intros; discriminate).
+   intros c'' H''.
+   case_eq (all_super_classes p c'' n); try (intros; discriminate).
+   intros.
+   inv H0.
+   destruct (subclass_left _ _ _ H2); auto.
+   destruct H0 as [c0 [T1 T2]].
+   clear H2.
+   inv T1.
+   unfold PROG.defined_Class in *.
+   assert (c0 = c'') by congruence.
+   assert (c'=CLASS.name c'') by congruence.
+   subst.
+   clear H2 H3 H1.
+   right; apply (IHn _ _ H H'' _ T2).
+
+   intros.
+   destruct (subclass_left _ _ _ H2); auto.
+   destruct H3 as [c0 [T1 T2]].
+   inv T1.
+   congruence.
+ Qed.
+
+ Fixpoint all_super_interfaces (p:Program) (n:nat) {struct n} : 
+                          Interface -> option (list Interface) :=
+   match n with
+     | O => fun _ => None
+     | S n => fun c =>
+       List.fold_left 
+         (fun o iname =>
+           match o with
+             | None => None
+             | Some l => 
+               match PROG.interface p iname with
+                 | None => None
+                 | Some itf => 
+                   match all_super_interfaces p n itf with
+                     | None => None
+                     | Some l' => Some (itf::l++l')
+                   end
+               end
+           end) 
+         (INTERFACE.superInterfaces c)
+         (Some (c::nil))
+   end.
+
+Lemma subinterface_left : forall p c1 c2,
+  subinterface p c1 c2 -> c1=c2 \/ (exists c, direct_subinterface p c1 c /\ subinterface p c c2).
+Proof.
+  intros p; unfold subinterface; apply clos_refl_trans_ind2; intros; auto.
+  destruct H1; subst; auto.
+  right; exists z; auto.
+  destruct H1 as [c [T1 T2]].
+  right; exists y; split; auto.
+Qed.
+
+Lemma all_super_interfaces_aux : forall p n l3,
+   fold_left
+     (fun (o : option (list Interface)) (iname : InterfaceName) =>
+      match o with
+      | Some l6 => 
+             match PROG.interface p iname with
+             | Some itf =>
+                 match all_super_interfaces p n itf with
+                 | Some l' => Some (itf :: l6 ++ l')
+                 | None => None (A:=list Interface)
+                 end
+             | None => None (A:=list Interface)
+             end
+      | None => None (A:=list Interface)
+      end) l3 None=None.
+Proof.
+  induction l3; simpl; auto.
+Qed.
+
+Lemma all_super_interfaces_aux' : forall p n l0 l1 l2,
+     fold_left
+        (fun (o : option (list Interface)) (iname : InterfaceName) =>
+         match o with
+         | Some l =>
+             match PROG.interface p iname with
+             | Some itf =>
+                 match all_super_interfaces p n itf with
+                 | Some l' => Some (itf :: l ++ l')
+                 | None => None (A:=list Interface)
+                 end
+             | None => None (A:=list Interface)
+             end
+         | None => None (A:=list Interface)
+         end) l0 (Some l1) = Some l2 -> incl l1 l2.
+Proof.
+  induction l0; simpl.
+  intros.
+  inversion H; subst; intro; auto.
+  destruct (PROG.interface p a); try (intros; discriminate).
+  destruct (all_super_interfaces p n i); try (intros; discriminate).
+  intros.
+  assert (IH:=IHl0 _ _ H); clear H IHl0.
+  repeat intro; apply IH.
+  right; auto with datatypes.
+  rewrite all_super_interfaces_aux; intros; discriminate.
+  rewrite all_super_interfaces_aux; intros; discriminate.
+ Qed.
+
+
+ Definition all_super_interfaces_correct : forall p n c l,
+   all_super_interfaces p n c = Some l ->
+   PROG.defined_Interface p c -> 
+   forall c', subinterface p c c' -> In c' (c::l).
+ Proof.
+   induction n; simpl.
+   intros; discriminate.
+   intros.
+   destruct (subinterface_left _ _ _ H1); clear H1; auto.
+   right; destruct H2 as [c0 [T1 T2]].
+   inv T1.
+   generalize dependent (Some (c::nil)).
+   generalize dependent (INTERFACE.superInterfaces c).
+   induction l0; simpl; intros.
+   elim H3.
+   destruct o; simpl in H; try discriminate.
+   case_eq (PROG.interface p a); intros.   
+   rewrite H4 in H.
+   case_eq (all_super_interfaces p n i); intros.
+   rewrite H5 in H.
+   destruct H3; subst.
+   unfold PROG.defined_Interface in *.
+   assert (c0=i) by congruence; clear H4; subst.
+   generalize (IHn _ _ H5 H2 _ T2).
+   assert (T:=all_super_interfaces_aux' _ _ _ _ _ H).
+   simpl; intros.
+   apply T.
+   destruct H3.
+   left; auto.
+   right; auto with datatypes.
+   apply IHl0 with (Some (i :: l1 ++ l2)); auto.
+   rewrite H5 in H.
+   rewrite all_super_interfaces_aux in H; discriminate.
+   rewrite H4 in H.
+   rewrite all_super_interfaces_aux in H; discriminate.
+   rewrite all_super_interfaces_aux in H; discriminate.
+ Qed.
+
+  Definition all_interfaces (p:Program) (n:nat) (c:Class) : option (list Interface) :=
+    List.fold_left 
+    (fun o iname =>
+      match o with
+        | None => None
+        | Some l => 
+          match PROG.interface p iname with
+            | None => None
+            | Some itf => 
+              match all_super_interfaces p n itf with
+                | None => None
+                | Some l' => Some (itf::l++l')
+              end
+          end
+      end) 
+    (CLASS.superInterfaces c)
+    (Some nil).
+
+  Lemma all_interfaces_correct : forall p n c l,
+    all_interfaces p n c = Some l -> forall i I I',
+      In i (CLASS.superInterfaces c) ->
+      PROG.interface p i = Some I ->
+      subinterface p I I' -> 
+      In I l.
+  Proof.
+    unfold all_interfaces.
+    intros p n c.
+    generalize (@nil Interface).
+    generalize (CLASS.superInterfaces c).
+    induction l; simpl.
+    intuition.
+    intros l0; case_eq (PROG.interface p a).
+    intros i Hi; case_eq (all_super_interfaces p n i); intros.
+    destruct H1; subst.
+    assert (I0=i) by congruence; subst; clear Hi.
+    apply (all_super_interfaces_aux' _ _ _ _ _ H0).
+    left; reflexivity.
+    eapply IHl ;eauto.
+    rewrite all_super_interfaces_aux in H0; discriminate.
+    intros.
+    rewrite all_super_interfaces_aux in H0; intros; discriminate.
+  Qed.
+
+
+
+Set Implicit Arguments.
+
+ Module Type HEAP.
+   Parameter t : Type.
+
+   Inductive AdressingMode : Set :=
+     | StaticField : FieldSignature -> AdressingMode
+     | DynamicField : Location -> FieldSignature -> AdressingMode
+     | ArrayElement : Location -> Z -> AdressingMode.
+
+   Inductive LocationType : Type :=
+     | LocationObject : ClassName -> LocationType  
+     | LocationArray : Int.t -> type -> Method*PC -> LocationType.
+   (** (LocationArray length element_type) *)
+
+   Parameter get : t -> AdressingMode -> option value.
+   Parameter update : t -> AdressingMode -> value -> t.
+   Parameter typeof : t -> Location -> option LocationType.   
+     (** typeof h loc = None -> no object, no array allocated at location loc *)
+   Parameter new : t -> Program -> LocationType -> option (Location * t).
+     (** program is required to compute the size of the allocated element, i.e. to know
+        the Class associated with a ClassName  *)
+
+   (** Compatibility between a heap and an adress *)
+   Inductive Compat (h:t) : AdressingMode -> Prop :=
+     | CompatStatic : forall f,
+         Compat h (StaticField f)
+     | CompatObject : forall cn loc f,
+         typeof h loc = Some (LocationObject cn) ->
+         Compat h (DynamicField loc f)
+     | CompatArray : forall length tp loc i a,
+         0 <= i < Int.toZ length ->
+         typeof h loc = Some (LocationArray length tp a) ->
+         Compat h (ArrayElement loc i).
+
+   Parameter get_update_same : forall h am v, Compat h am ->  get (update h am v) am = Some v.
+   Parameter get_update_old : forall h am1 am2 v, am1<>am2 -> get (update h am1 v) am2 = get h am2.
+   Parameter get_uncompat : forall h am, ~ Compat h am -> get h am = None.
+
+   Parameter typeof_update_same : forall h loc am v,
+     typeof (update h am v) loc = typeof h loc.
+
+   Parameter new_fresh_location : forall (h:t) (p:Program) (lt:LocationType) (loc:Location) (h':t),
+     new h p lt = Some (loc,h') ->
+     typeof h loc = None.
+
+   Parameter new_typeof : forall (h:t) (p:Program) (lt:LocationType) (loc:Location) (h':t),
+     new h p lt = Some (loc,h') ->
+     typeof h' loc = Some lt.
+
+   Parameter new_typeof_old : forall (h:t) (p:Program) (lt:LocationType) (loc loc':Location) (h':t),
+     new h p lt = Some (loc,h') ->
+     loc <> loc' ->
+     typeof h' loc' = typeof h loc'.
+
+   Parameter new_defined_object_field : forall (h:t) (p:Program) (cn:ClassName) (fs:FieldSignature) (f:Field) (loc:Location) (h':t), 
+     new h p (LocationObject cn) = Some (loc,h') ->
+     is_defined_field p cn fs f ->
+     get h' (DynamicField loc fs) = Some (init_field_value f).
+
+   Parameter new_undefined_object_field : forall (h:t) (p:Program) (cn:ClassName) (fs:FieldSignature) (loc:Location) (h':t),
+     new h p (LocationObject cn) = Some (loc,h') ->
+     ~ defined_field p cn fs ->
+     get h' (DynamicField loc fs) = None.
+ 
+  Parameter new_object_no_change : 
+     forall (h:t) (p:Program) (cn:ClassName) (loc:Location) (h':t) (am:AdressingMode),
+     new h p (LocationObject cn) = Some (loc,h') ->
+     (forall (fs:FieldSignature), am <> (DynamicField loc fs)) ->
+     get h' am = get h am.
+
+  Parameter new_valid_array_index : forall (h:t) (p:Program) (length:Int.t) (tp:type) a (i:Z) (loc:Location) (h':t),
+     new h p (LocationArray length tp a) = Some (loc,h') ->
+     0 <= i < Int.toZ length ->
+     get h' (ArrayElement loc i) = Some (init_value tp).
+
+  Parameter new_unvalid_array_index : forall (h:t) (p:Program) (length:Int.t) (tp:type) a (i:Z) (loc:Location) (h':t),
+     new h p (LocationArray length tp a) = Some (loc,h') ->
+     ~ 0 <= i < Int.toZ length ->
+     get h' (ArrayElement loc i) = None.
+
+  Parameter new_array_no_change : 
+     forall (h:t) (p:Program) (length:Int.t) (tp:type) a (loc:Location) (h':t) (am:AdressingMode),
+     new h p (LocationArray length tp a) = Some (loc,h') ->
+     (forall (i:Z), am <> (ArrayElement loc i)) ->
+     get h' am = get h am.
+
+(* These properties should be useless
+   Parameter get_static_some : forall (h:t) (p:Program) (fs:FieldSignature),
+     isStatic p fs ->
+     exists v, get h (StaticField fs) = Some v.
+
+   Parameter get_static_some : forall (h:t) (p:Program) (fs:FieldSignature),
+     ~ isStatic p fs ->
+     exists v, get h (StaticField fs) = None.
+*)
+
+ End HEAP.
+
+Module Heap <: HEAP.
+  Module Object.
+    Record t : Type := Obj { class : ClassName; fieldsval : MapFieldSignature.t value }.
+    Definition get (o:t) := MapFieldSignature.get value o.(fieldsval).
+    Definition op_get (o:option t) :=
+      match o with
+        | Some o => get o
+        | None => fun f => None
+      end.
+    Definition op_update (f:FieldSignature) (v:value) (o:option t) : option t :=
+      match o with
+        | None => None
+        | Some o => Some (Obj o.(class) (MapFieldSignature.update _ o.(fieldsval) f v))
+      end.
+
+    Definition init_fields :  list (ClassName*Field) -> MapFieldSignature.t value :=
+      @fold_right (MapFieldSignature.t value) _
+        (fun f m => MapFieldSignature.update _ m (fst f,FIELD.signature (snd f)) (init_field_value (snd f)))
+        (MapFieldSignature.empty _).
+
+    Definition default (c:Class) : t :=
+      Obj
+      (CLASS.name c) 
+      (init_fields (List.map (fun f => (CLASS.name c,f)) (CLASS.definedFields c))).
+
+  End Object.
+  Module Array.
+    Record t : Type := Arr {
+      length : Int.t;
+      element_type : type; 
+      elements : BinNatMap.t value;
+      creation_point : Method * PC
+    }.
+
+    Definition Ncase (i:Z)  : option N :=
+      match i with
+        | Z0 => Some N0
+        | Zpos p => Some (Npos p)
+        | _ => None
+      end.
+
+    Definition get (a:t) (i:Z) :=
+      match Ncase i with
+        | Some n => 
+          match Zcompare i (Int.toZ a.(length)) with
+            | Lt => BinNatMap.get value a.(elements) n
+            | _ => None
+          end
+        | None => None
+      end.
+    Definition op_get (a:option (t)) :=
+      match a with
+        | Some a => get a
+        | None => fun i => None
+      end.
+    Definition op_update (i:Z) (v:value) (a:option t) : option t :=
+      match a with
+        | None => None
+        | Some a => 
+          match Ncase i with
+            | Some n =>
+              match Zcompare i (Int.toZ a.(length)) with
+                | Lt => Some 
+                         (Arr a.(length) a.(element_type) (BinNatMap.update _ a.(elements) n v) a.(creation_point))
+                | _ => Some a
+              end
+            | _ => Some a
+          end
+      end.
+
+    Fixpoint init_array_rec (n:nat) (v:value) {struct n} : BinNatMap.t value :=
+      match n with 
+        | O => BinNatMap.empty _
+        | S p => BinNatMap.update _ (init_array_rec p v) (N_of_nat p) v
+      end.
+
+    Definition default (lgth:Int.t) (n:nat) (tp:type) (a:Method*PC): t:=
+      Arr lgth tp (init_array_rec n (init_value tp)) a.
+
+   Definition N_to_nat (n:N) : nat :=
+     match n with
+       | Npos p => nat_of_P p
+       | N0 => O
+     end.
+ 
+   Lemma ZL4_inf : forall y:positive, {h : nat | nat_of_P y = S h}.
+   Proof.
+   intro y; induction y as [p H| p H1| ];
+    [ elim H; intros x H1; exists (S x + S x)%nat; unfold nat_of_P in |- *; simpl in |- *; rewrite ZL0; rewrite Pmult_nat_r_plus_morphism; unfold nat_of_P in H1; rewrite H1; auto with arith | elim H1; intros x H2; exists (x + S x)%nat; unfold nat_of_P in |- *; simpl in |- *; rewrite ZL0; rewrite Pmult_nat_r_plus_morphism; unfold nat_of_P in H2; rewrite H2; auto with arith | exists 0%nat; auto with arith ].
+   Qed.
+
+   Lemma N_of_nat_N_to_nat : forall n, N_of_nat (N_to_nat n) = n.
+   Proof.
+     unfold N_of_nat, N_to_nat; intros.
+     destruct n.
+     reflexivity.
+     destruct (ZL4_inf p).
+     rewrite e.
+     generalize (nat_of_P_o_P_of_succ_nat_eq_succ x).
+     rewrite <- e; intros.
+     assert (Zpos (P_of_succ_nat x) = Zpos p).
+     rewrite Zpos_eq_Z_of_nat_o_nat_of_P.
+     rewrite H.
+     rewrite Zpos_eq_Z_of_nat_o_nat_of_P.
+     auto.
+     congruence.
+   Qed.
+
+   Lemma N_to_nat_N_of_nat : forall n, N_to_nat (N_of_nat n) = n.
+   Proof.
+     unfold N_of_nat, N_to_nat; intros.
+     destruct n.
+     reflexivity.
+     rewrite nat_of_P_o_P_of_succ_nat_eq_succ.
+     reflexivity.
+   Qed.
+
+   Lemma get_init_array_rec: forall n v i,
+      (N_to_nat i<n)%nat ->
+      BinNatMap.get _ (init_array_rec n v) i = Some v.
+   Proof.
+     induction n; simpl; intros.
+     apply False_ind; omega.
+     assert (N_to_nat i < n \/ N_to_nat i = n)%nat by omega.
+     destruct H0; clear H.
+     rewrite BinNatMap.get_update2.
+     auto.
+     intro; subst.
+     rewrite N_to_nat_N_of_nat in H0; omega.
+     subst.
+     rewrite N_of_nat_N_to_nat.
+     rewrite BinNatMap.get_update1.
+     reflexivity.
+   Qed.
+
+   Lemma get_init_array_none_rec: forall n v i,
+      (N_to_nat i>=n)%nat ->
+      BinNatMap.get _ (init_array_rec n v) i = None.
+   Proof.
+     induction n; simpl; intros.
+     apply BinNatMap.get_empty.
+     rewrite BinNatMap.get_update2.
+     apply IHn.
+     omega.
+     intro; subst.
+     rewrite N_to_nat_N_of_nat in H; omega.
+   Qed.
+
+
+  End Array.
+
+  Module LocMap := BinNatMap.
+
+  Record t_ : Type := hp {
+    statics : MapFieldSignature.t value;
+    objects : LocMap.t Object.t;
+    arrays : LocMap.t Array.t;
+    next_loc : Location
+  }.
+  Definition t : Type := t_.
+  
+  Inductive AdressingMode : Set :=
+  | StaticField : FieldSignature -> AdressingMode
+  | DynamicField : Location -> FieldSignature -> AdressingMode
+  | ArrayElement : Location -> Z -> AdressingMode.
+
+  Inductive LocationType : Type :=
+  | LocationObject : ClassName -> LocationType 
+  | LocationArray : Int.t -> type -> Method*PC -> LocationType.
+
+   Definition typeof (h:t) (l:Location) : option (LocationType) :=
+     match LocMap.get _ h.(objects) l with
+       | Some o => Some (LocationObject o.(Object.class))
+       | None =>
+         match LocMap.get _ h.(arrays) l with
+           | Some a => Some (LocationArray a.(Array.length) a.(Array.element_type) a.(Array.creation_point))
+           | None => None
+         end
+     end.
+
+   (** Compatibility between a heap and an adress *)
+   Inductive Compat (h:t) : AdressingMode -> Prop :=
+     | CompatStatic : forall f,
+         Compat h (StaticField f)
+     | CompatObject : forall cn loc f,
+         typeof h loc = Some (LocationObject cn) ->
+         Compat h (DynamicField loc f)
+     | CompatArray : forall length tp loc i a,
+         0 <= i < Int.toZ length ->
+         typeof h loc = Some (LocationArray length tp a) ->
+         Compat h (ArrayElement loc i).
+
+   Definition check_compat (h:t) (am:AdressingMode) : bool :=
+     match am with
+       | StaticField f => true
+       | DynamicField loc f =>
+         match typeof h loc with
+           | Some (LocationObject _) => true
+           | _ => false
+         end
+       | ArrayElement loc i =>
+         match typeof h loc with
+           | Some (LocationArray length _ _ ) => 
+             match i ?= 0 with
+               | Lt => false
+               | _ =>
+                 match i ?= Int.toZ length with
+                   | Lt => true
+                   | _ => false
+                 end
+             end
+           | _ => false
+         end
+     end.
+
+   Lemma bounded_compare : forall i t:Z,
+     i < t -> i ?= t = Lt.
+   Proof.
+     intros.
+     generalize (Zlt_compare _ _ H); rewrite H; auto.
+   Qed.
+
+   Lemma case_compare : forall i t:Z,
+     (i ?= t = Lt /\ i<t) \/ (i ?=t = Gt) \/ (i ?=t = Eq).
+   Proof.
+     intros.
+     generalize (Zge_compare i t0).
+     destruct (i ?= t0); simpl; auto.
+     left; split; auto; omega.
+   Qed.
+
+   Lemma check_compat_correct : forall h am,
+     if check_compat h am then Compat h am else ~ Compat h am.
+   Proof.
+     unfold check_compat; intros.
+     destruct am.
+     constructor.
+     case_eq (typeof h l); intros.
+     destruct l0.
+     econstructor; eauto.
+     intro T; inversion T; subst.
+     rewrite H1 in H; discriminate.
+     intro T; inversion T; subst.
+     rewrite H1 in H; discriminate.
+     case_eq (typeof h l); intros.
+     destruct l0.
+     intro T; inversion T; subst.
+     rewrite H3 in H; discriminate.
+     generalize (Zge_compare z 0).
+     generalize (Zlt_compare z 0).
+     destruct (z ?= 0).
+     generalize (Zge_compare z (Int.toZ t0)).
+     generalize (Zlt_compare z (Int.toZ t0)).
+     destruct (z ?= (Int.toZ t0)).
+     repeat intro.
+     inversion H4; subst.
+     rewrite H8 in H; inversion H; subst; omega.
+     intros; econstructor; eauto.
+     omega.
+     repeat intro.
+     inversion H4; subst.
+     rewrite H8 in H; inversion H; subst; omega.
+     repeat intro.
+     inversion H2; subst.
+     rewrite H6 in H; inversion H; subst; omega.
+     generalize (Zge_compare z (Int.toZ t0)).
+     generalize (Zlt_compare z (Int.toZ t0)).
+     destruct (z ?= (Int.toZ t0)).
+     repeat intro.
+     inversion H4; subst.
+     rewrite H8 in H; inversion H; subst; omega.
+     intros; econstructor; eauto.
+     omega.
+     repeat intro.
+     inversion H4; subst.
+     rewrite H8 in H; inversion H; subst; omega.
+     intro.
+     inversion H0; subst.
+     rewrite H4 in H; inversion H.
+   Qed.
+
+  Definition get (h:t) (am:AdressingMode) : option value :=
+    if check_compat h am then
+      match am with
+        | StaticField f =>  MapFieldSignature.get _ h.(statics) f
+        | DynamicField l f => Object.op_get (LocMap.get _ h.(objects) l) f
+        | ArrayElement l i => Array.op_get (LocMap.get _ h.(arrays) l) i 
+      end
+      else None.
+  Definition update (h:t) (am:AdressingMode) (v:value) : t :=
+    if check_compat h am then
+      match am with
+        | StaticField f => 
+          hp
+          (MapFieldSignature.update _ h.(statics) f v)
+          h.(objects)
+          h.(arrays)
+          h.(next_loc)
+        | DynamicField l f => 
+          hp
+          h.(statics)
+          (LocMap.modify _ h.(objects) l (Object.op_update f v))
+          h.(arrays)              
+          h.(next_loc)
+        | ArrayElement l i => 
+          hp
+          h.(statics)
+          h.(objects)
+          (LocMap.modify _ h.(arrays) l (Array.op_update i v))
+          h.(next_loc)
+      end else h.     
+
+   Definition Int_to_nat (i:Int.t) : option nat :=
+     match Int.toZ i with
+       | Zpos p => Some (nat_of_P p)
+       | Z0 => Some O
+       | Zneg _ => None
+     end.
+
+   Definition check_fresh (h:t) (l:Location) : bool :=
+     match LocMap.get _ h.(objects) l with
+       | Some _ => false
+       | _ =>      
+         match LocMap.get _ h.(arrays) l with
+           | Some _ => false
+           | _ => true
+         end
+     end.
+
+   Lemma check_fresh_correct : forall h l,
+     check_fresh h l = true ->
+       (LocMap.get _ h.(objects) l = None
+        /\ LocMap.get _ h.(arrays) l = None).
+   Proof.
+     unfold check_fresh; intros.
+     destruct (LocMap.get _ (objects h) l); try discriminate.
+     destruct (LocMap.get _ (arrays h) l); try discriminate.
+     auto.
+   Qed.
+
+   Definition new (h:t) (p:Program) (ltp:LocationType) : option (Location * t) :=
+     if check_fresh h h.(next_loc) then
+       match ltp with
+         | LocationObject cn => 
+           match PROG.class p cn with
+             | None => None
+             | Some c => 
+                 Some
+                 (h.(next_loc),
+                   hp
+                   h.(statics)
+                   (LocMap.update _ h.(objects) h.(next_loc) (Object.default c))
+                   h.(arrays)              
+                   (Nsucc h.(next_loc)))
+           end
+       | LocationArray lgth tp a => 
+             match Int_to_nat lgth with
+               | None => None
+               | Some n =>
+                 Some
+                 (h.(next_loc),
+                   hp
+                   h.(statics)
+                   h.(objects)              
+                   (LocMap.update _ h.(arrays) h.(next_loc) (Array.default lgth n tp a))
+                   (Nsucc h.(next_loc)))
+             end
+       end
+       else None.
+
+   Lemma pos_Ncase : forall i:Z,
+     0<=i -> exists n, Array.Ncase i = Some n.
+   Proof.
+     destruct i; simpl; intros; eauto.
+     elim H; auto.
+   Qed.
+
+   Lemma case_Ncase : forall i:Z,
+     Array.Ncase i = None \/
+     exists n, Array.Ncase i = Some n /\ 0<=i.
+   Proof.
+     destruct i; simpl; eauto with zarith.
+   Qed.
+
+   Lemma Ncase_inj : forall i j,
+     Array.Ncase i = Array.Ncase j -> Array.Ncase i <> None -> i = j.
+   Proof.
+     destruct i; destruct j; intros H; inversion H; auto.
+     simpl; intuition.
+   Qed.
+
+   Lemma typeof_update_same : forall h loc am v,
+     typeof (update h am v) loc = typeof h loc.
+   Proof.
+     unfold typeof, update; intros.
+     generalize (check_compat_correct h am); destruct (check_compat h am); simpl; intros.
+     destruct H; simpl.
+     auto.
+     destruct (PC_eq_dec loc0 loc); subst.
+     unfold typeof in H.
+     rewrite LocMap.get_modify1; auto.
+     unfold LocMap.get in H.
+     unfold LocMap.get in *.
+     case_eq (BinNatMap_Base.get Object.t (objects h) loc); intros.
+     rewrite H0 in H.
+     reflexivity.
+     rewrite H0 in H.
+     reflexivity.
+     
+     rewrite LocMap.get_modify2; auto.
+
+     destruct (PC_eq_dec loc0 loc); subst.
+     rewrite LocMap.get_modify1; auto.
+     unfold typeof in *.
+     destruct (LocMap.get Object.t (objects h) loc); try reflexivity.
+     unfold LocMap.get in *.
+     case_eq (BinNatMap_Base.get _ (arrays h) loc); simpl; intros.
+     rewrite H1 in H0.
+     inversion H0; clear H0; subst.
+     elim (@pos_Ncase i); [intros n H2|omega].
+     rewrite H2.
+     rewrite bounded_compare; try omega.
+     reflexivity.
+     reflexivity.
+     rewrite LocMap.get_modify2; auto.
+
+     reflexivity.
+   Qed.
+
+   Lemma Compat_update1 : forall h am am0 v0,
+     Compat h am -> Compat (update h am0 v0) am.
+   Proof.
+     destruct 1; econstructor; eauto.
+     rewrite typeof_update_same; eauto.
+     rewrite typeof_update_same; eauto.
+   Qed.
+
+   Lemma Compat_update2 : forall h am am0 v0,
+     Compat (update h am0 v0) am -> Compat h am.
+   Proof.
+     destruct 1; econstructor; eauto.
+     rewrite typeof_update_same in H; eauto.
+     rewrite typeof_update_same in H0; eauto.
+   Qed.
+
+   Lemma check_compat_update : forall h am v am',
+     check_compat (update h am v) am' = check_compat h am'.
+   Proof.
+     intros.
+     generalize (check_compat_correct (update h am v) am').
+     generalize (check_compat_correct h am').
+     destruct (check_compat (update h am v) am');
+     destruct (check_compat h am'); auto.
+     intros.
+     elim H; eapply Compat_update2; eauto.
+     intros.
+     elim H0; eapply Compat_update1; eauto.   
+   Qed.
+
+   Lemma get_update_same : forall h am v, Compat h am ->  get (update h am v) am = Some v.
+   Proof.
+     unfold get; intros.
+     rewrite check_compat_update.
+     unfold update.
+     generalize (check_compat_correct h am); destruct (check_compat h am).
+     clear H.     
+     destruct 1; simpl.
+     rewrite MapFieldSignature.get_update1; auto.
+     rewrite LocMap.get_modify1; auto.
+     caseeq (BinNatMap_Base.get Object.t (objects h) loc); intros; simpl.
+     unfold Object.get; simpl.
+     rewrite MapFieldSignature.get_update1; auto.
+     unfold typeof in H.
+     replace LocMap.get with BinNatMap_Base.get in H; auto.
+     rewrite H0 in H.
+     destruct (BinNatMap_Base.get (Array.t) (arrays h) loc); discriminate.
+
+     unfold typeof in H0.
+     replace LocMap.get with BinNatMap_Base.get in *; auto.
+     caseeq (BinNatMap_Base.get Object.t (objects h) loc); intros; simpl.
+     rewrite H1 in H0.
+     inversion H0.
+     rewrite H1 in *.
+     rewrite LocMap.get_modify1; auto.
+     unfold Array.op_update, Array.op_get, Array.get.
+     caseeq (BinNatMap_Base.get _ (arrays h) loc); intros.
+     rewrite H2 in H0.
+     injection H0; intros; subst; clear H0.
+     destruct (Array.elements t0).
+     elim (@pos_Ncase i); [intros n Hn|omega].
+     rewrite Hn.
+     rewrite bounded_compare; [idtac|omega].
+     rewrite Hn.
+     simpl.
+     rewrite bounded_compare; [idtac|omega].
+     destruct n; simpl; auto.
+     rewrite BinMap_Base.get_modify1; auto.
+     rewrite H2 in H0; discriminate.
+     intuition.
+   Qed.
+
+   Lemma get_update_old : forall h am1 am2 v, am1<>am2 -> get (update h am1 v) am2 = get h am2.
+   Proof.
+     unfold get; intros.
+     rewrite check_compat_update.
+     unfold update; intros.
+     generalize (check_compat_correct h am1); destruct (check_compat h am1); auto.
+     destruct 1; destruct am2; simpl; intros; auto.
+     rewrite MapFieldSignature.get_update2; auto; congruence.
+
+     destruct (PC_eq_dec loc l); subst.
+     rewrite LocMap.get_modify1; auto.
+     unfold typeof,LocMap.get in *.
+     destruct (BinNatMap_Base.get Object.t (objects h) l); simpl in *.
+     unfold Object.get; simpl.
+     rewrite MapFieldSignature.get_update2; auto; congruence.
+     auto.
+     rewrite LocMap.get_modify2; auto.
+
+     destruct (PC_eq_dec loc l); subst.
+     unfold typeof in H1.
+     caseeq (LocMap.get _ (objects h) l); intros; simpl; auto.
+     rewrite H2 in H1; inversion H1.
+     rewrite H2 in H1.
+     unfold LocMap.get in *.
+     rewrite LocMap.get_modify1; auto.
+     clear H2.
+     caseeq (BinNatMap_Base.get Array.t (arrays h) l); intros; simpl; auto.
+     rewrite H2 in H1; try discriminate.
+     inversion H1; subst; clear H1.
+     destruct (case_Ncase i).
+     rewrite H1; auto.
+     destruct H1 as [n [H1 H3]]; rewrite H1.
+     destruct (case_compare i (Int.toZ (Array.length t0))).
+     destruct H4 as [H4 H5]; rewrite H4.
+     simpl.
+     unfold Array.get.
+     destruct (case_Ncase z).
+     rewrite H6; auto.
+     destruct H6 as [n' [H6 H7]]; rewrite H6; simpl.
+     destruct (case_compare z (Int.toZ (Array.length t0))).
+     destruct H8 as [H8 H9]; rewrite H8.
+     rewrite BinNatMap.get_update2; auto.
+     intro; assert (i=z) by (apply Ncase_inj; congruence).
+     elim H; congruence.
+     destruct H8; rewrite H8; auto.
+     destruct H4; rewrite H4; auto.
+     rewrite LocMap.get_modify2; auto.
+   Qed.
+     
+   Lemma get_uncompat : forall h am, ~ Compat h am -> get h am = None.
+   Proof.
+     unfold get; intros.
+     generalize (check_compat_correct h am);
+       destruct (check_compat h am); intuition.
+   Qed.
+
+   Lemma new_fresh_location : forall (h:t) (p:Program) (lt:LocationType) (loc:Location) (h':t),
+     new h p lt = Some (loc,h') ->
+     typeof h loc = None.
+   Proof.
+     unfold new; intros.
+     generalize (check_fresh_correct h (next_loc h)).
+     destruct (check_fresh h (next_loc h)); try discriminate.
+     intros T; destruct (T (refl_equal _)); clear T.
+     unfold typeof; destruct lt.
+     destruct (PROG.class p c); try discriminate.
+     inversion H; clear H; subst.
+     rewrite H0; rewrite H1; reflexivity.
+     destruct (Int_to_nat t0); try discriminate.
+     inversion H; clear H; subst.
+     rewrite H0; rewrite H1; reflexivity.
+   Qed.
+     
+   Lemma new_typeof : forall (h:t) (p:Program) (lt:LocationType) (loc:Location) (h':t),
+     new h p lt = Some (loc,h') ->
+     typeof h' loc = Some lt.
+   Proof.
+     unfold new, typeof; intros.
+     assert (T:=check_fresh_correct h (next_loc h)).
+     destruct (check_fresh h (next_loc h)); try discriminate.
+     destruct lt.
+     case_eq (PROG.class p c); intros.
+     rewrite H0 in H.
+     inversion H; clear H; subst.
+     simpl.
+     rewrite LocMap.get_update1.
+     generalize (PROG.name_class_invariant1 _ _ _ H0).
+     unfold Object.default; simpl.
+     intros; congruence.
+     rewrite H0 in H; discriminate.
+     destruct (Int_to_nat t0); inversion H; clear H; subst; simpl.
+     destruct (T (refl_equal _)) as [T1 T2]; clear T.
+     rewrite T1.
+     rewrite LocMap.get_update1.
+     reflexivity.
+   Qed.
+
+   Lemma new_typeof_old : forall (h:t) (p:Program) (lt:LocationType) (loc loc':Location) (h':t),
+     new h p lt = Some (loc,h') ->
+     loc <> loc' ->
+     typeof h' loc' = typeof h loc'.
+   Proof.
+     unfold new, typeof; intros.
+     assert (T:=check_fresh_correct h (next_loc h)).
+     destruct (check_fresh h (next_loc h)); try discriminate.
+     destruct (T (refl_equal _)) as [T1 T2]; clear T.
+     destruct lt.
+     destruct (PROG.class p c); try discriminate.
+     inversion H; clear H; subst.
+     simpl.
+     rewrite LocMap.get_update2; auto.
+     destruct (Int_to_nat t0); inversion H; clear H; subst; simpl.
+     rewrite LocMap.get_update2; auto.
+   Qed.
+
+   Lemma Compat_new_obj1 :
+     forall (h:t) (p:Program) (cn:ClassName) (loc:Location) (h':t) (am:AdressingMode),
+     new h p (LocationObject cn) = Some (loc,h') ->
+     Compat h am -> Compat h' am.
+   Proof.
+     intros.
+     destruct H0; econstructor; eauto.
+     rewrite (@new_typeof_old _ _ _ _ loc0 _ H); eauto.
+     intro; subst.
+     rewrite (@new_fresh_location _ _ _ _ _ H) in H0.
+     discriminate.
+     rewrite (@new_typeof_old _ _ _ _ loc0 _ H); eauto.
+     intro; subst.
+     rewrite (@new_fresh_location _ _ _ _ _ H) in H1.
+     discriminate.     
+   Qed.
+
+   Lemma Compat_new_obj2 :
+     forall (h:t) (p:Program) (cn:ClassName) (loc:Location) (h':t) (am:AdressingMode),
+     new h p (LocationObject cn) = Some (loc,h') ->
+     (forall (fs:FieldSignature), am <> (DynamicField loc fs)) ->
+     Compat h' am -> Compat h am.
+   Proof.
+     intros.
+     destruct H1; econstructor; eauto.
+     rewrite (@new_typeof_old _ _ _ _ loc0 _ H) in H1; eauto.
+     intro; subst.
+     elim (H0 f); auto.
+     rewrite (@new_typeof_old _ _ _ _ loc0 _ H) in H2; eauto.
+     intro; subst.
+     rewrite (@new_typeof _ _ _ _ _ H) in H2.
+     discriminate.     
+   Qed.
+
+   Lemma check_compat_new_obj :
+     forall (h:t) (p:Program) (cn:ClassName) (loc:Location) (h':t) (am:AdressingMode),
+     new h p (LocationObject cn) = Some (loc,h') ->
+     (forall (fs:FieldSignature), am <> (DynamicField loc fs)) ->
+     check_compat h' am = check_compat h am.
+   Proof.
+     intros.
+     generalize (check_compat_correct h' am).
+     generalize (check_compat_correct h am).
+     destruct (check_compat h' am);
+     destruct (check_compat h am); auto.
+     intros.
+     elim H1; eapply Compat_new_obj2; eauto.
+     intros.
+     elim H2; eapply Compat_new_obj1; eauto.   
+   Qed.
+
+   Lemma Compat_new_array1 :
+     forall (h:t) (p:Program) i tp a (loc:Location) (h':t) (am:AdressingMode),
+     new h p (LocationArray i tp a) = Some (loc,h') ->
+     Compat h am -> Compat h' am.
+   Proof.
+     intros.
+     destruct H0; econstructor; eauto.
+     rewrite (@new_typeof_old _ _ _ _ loc0 _ H); eauto.
+     intro; subst.
+     rewrite (@new_fresh_location _ _ _ _ _ H) in H0.
+     discriminate.
+     rewrite (@new_typeof_old _ _ _ _ loc0 _ H); eauto.
+     intro; subst.
+     rewrite (@new_fresh_location _ _ _ _ _ H) in H1.
+     discriminate.     
+   Qed.
+
+   Lemma Compat_new_array2 :
+     forall (h:t) (p:Program) i tp a (loc:Location) (h':t) (am:AdressingMode),
+     new h p (LocationArray i tp a) = Some (loc,h') ->
+     (forall j, am <> (ArrayElement loc j)) ->
+     Compat h' am -> Compat h am.
+   Proof.
+     intros.
+     destruct H1; econstructor; eauto.
+     rewrite (@new_typeof_old _ _ _ _ loc0 _ H) in H1; eauto.
+     intro; subst.
+     rewrite (@new_typeof _ _ _ _ _ H) in H1.
+     discriminate.
+     rewrite (@new_typeof_old _ _ _ _ loc0 _ H) in H2; eauto.
+     intro; subst.
+     elim (H0 i0); auto.
+   Qed.
+
+   Lemma check_compat_new_array :
+     forall (h:t) (p:Program) i tp a (loc:Location) (h':t) am,
+     new h p (LocationArray i tp a) = Some (loc,h') ->
+     (forall j, am <> (ArrayElement loc j)) ->
+     check_compat h' am = check_compat h am.
+   Proof.
+     intros.
+     generalize (check_compat_correct h' am).
+     generalize (check_compat_correct h am).
+     destruct (check_compat h' am);
+     destruct (check_compat h am); auto.
+     intros.
+     elim H1; eapply Compat_new_array2; eauto.
+     intros.
+     elim H2; eapply Compat_new_array1; eauto.   
+   Qed.
+
+   Parameter new_defined_object_field : forall (h:t) (p:Program) (cn:ClassName) (fs:FieldSignature) (f:Field) (loc:Location) (h':t),
+     new h p (LocationObject cn) = Some (loc,h') ->
+     is_defined_field p cn fs f ->
+     get h' (DynamicField loc fs) = Some (init_field_value f).
+
+   Axiom new_undefined_object_field : forall (h:t) (p:Program) (cn:ClassName) (fs:FieldSignature) (loc:Location) (h':t),
+     new h p (LocationObject cn) = Some (loc,h') ->
+     ~ defined_field p cn fs ->
+     get h' (DynamicField loc fs) = None.
+ 
+  Lemma new_object_no_change : 
+     forall (h:t) (p:Program) (cn:ClassName) (loc:Location) (h':t) (am:AdressingMode),
+     new h p (LocationObject cn) = Some (loc,h') ->
+     (forall (fs:FieldSignature), am <> (DynamicField loc fs)) ->
+     get h' am = get h am.
+   Proof.
+     unfold get; intros.
+     rewrite (@check_compat_new_obj _ _ _ _ _ _ H H0).
+     assert (T:=check_compat_correct h am).
+     destruct (check_compat h am); try reflexivity.
+     unfold new in *.
+     destruct (check_fresh h (next_loc h)); try discriminate.
+     destruct (PROG.class p cn); try discriminate.
+     inversion H; clear H; subst.
+     destruct T; simpl.
+     reflexivity.
+     rewrite LocMap.get_update2; auto.
+     intro; subst; elim (H0 f); auto.
+     auto.
+   Qed.
+
+  Lemma new_valid_array_index : forall (h:t) (p:Program) (length:Int.t) (tp:type) a (i:Z) (loc:Location) (h':t),
+     new h p (LocationArray length tp a) = Some (loc,h') ->
+     0 <= i < Int.toZ length ->
+     get h' (ArrayElement loc i) = Some (init_value tp).
+   Proof.
+     unfold get; intros.
+     assert (T:=check_compat_correct h' (ArrayElement loc i)).
+     destruct (check_compat h' (ArrayElement loc i)).
+     unfold new in *; simpl.
+     destruct (check_fresh h (next_loc h)); try discriminate.
+     assert (exists p, Int.toZ length = Zpos p).
+     destruct (Int.toZ length); eauto.
+     apply False_ind; omega.
+     generalize (Zlt_neg_0 p0); intros.
+     apply False_ind; omega.
+     destruct H1.
+     unfold Int_to_nat in H; rewrite H1 in H.
+     inversion H; clear H; subst.
+     simpl.
+     rewrite LocMap.get_update1.
+     simpl.
+     unfold Array.default; simpl.
+     unfold Array.get; simpl.
+     unfold Array.Ncase.
+     rewrite H1.
+     rewrite bounded_compare.
+     destruct i.
+     apply Array.get_init_array_rec. 
+     simpl.
+     apply lt_O_nat_of_P.
+     apply Array.get_init_array_rec. 
+     simpl.
+     apply nat_of_P_lt_Lt_compare_morphism.
+     generalize (Zlt_compare (Zpos p0) (Zpos x)).
+     simpl. 
+      intros. inversion H0. rewrite H1 in H3. apply H3.
+     generalize (Zlt_neg_0 p0); intros. omega.
+     omega. 
+     elim T; econstructor; eauto.
+     eapply new_typeof; eauto.
+   Qed.
+
+  Lemma new_unvalid_array_index : forall (h:t) (p:Program) (length:Int.t) (tp:type) a (i:Z) (loc:Location) (h':t),
+     new h p (LocationArray length tp a) = Some (loc,h') ->
+     ~ 0 <= i < Int.toZ length ->
+     get h' (ArrayElement loc i) = None.
+  Proof.
+     unfold get; intros.
+     assert (T:=check_compat_correct h' (ArrayElement loc i)).
+     destruct (check_compat h' (ArrayElement loc i)).
+     unfold new in *; simpl.
+     destruct (check_fresh h (next_loc h)); try discriminate.
+     unfold Array.op_get, Array.get.
+     inversion T; clear T; subst.
+     case_eq (Int_to_nat length); intros.
+     rewrite H1 in H; try discriminate.
+     inversion H; clear H; subst.
+     simpl.
+     rewrite LocMap.get_update1.
+     elim (@pos_Ncase  i); [intros|omega].
+     rewrite H.
+     simpl.
+     unfold typeof in H4.
+     simpl in H4.
+     destruct (LocMap.get Object.t (objects h) (next_loc h)); try discriminate.
+     rewrite LocMap.get_update1 in H4.
+     inversion H4; clear H4; subst.
+     elim H0; auto.
+     rewrite H1 in H; discriminate.
+     reflexivity.
+   Qed.
+
+  Lemma new_array_no_change : 
+     forall (h:t) (p:Program) (length:Int.t) (tp:type) a (loc:Location) (h':t) (am:AdressingMode),
+     new h p (LocationArray length tp a) = Some (loc,h') ->
+     (forall (i:Z), am <> (ArrayElement loc i)) ->
+     get h' am = get h am.
+  Proof.
+     unfold get; intros.
+     rewrite (@check_compat_new_array _ _ _ _ _ _ _ _ H H0).
+     assert (T:=check_compat_correct h am).
+     destruct (check_compat h am); try reflexivity.
+     unfold new in *.
+     destruct (check_fresh h (next_loc h)); try discriminate.
+     destruct (Int_to_nat length); try discriminate.
+     inversion H; clear H; subst.
+     destruct T; simpl.
+     reflexivity.
+     reflexivity.
+     rewrite LocMap.get_update2; auto.
+     intro; subst; elim (H0 i); auto.
+   Qed.
+
+ End Heap.
+
+Opaque Heap.update.
+  Inductive ReturnVal : Set :=
+   | Normal : option value -> ReturnVal
+   | Exception : Location -> ReturnVal.
+
+ (** Domain of frames *)
+ Module Type FRAME.
+   Inductive t : Type := 
+      make : Method -> PC -> (*OperandStack.t ->*) LocalVar.t -> t.
+ End FRAME.
+ 
+ Module Frame.
+   Inductive t : Type := 
+      make : Method -> PC -> (*OperandStack.t ->*) LocalVar.t -> t.
+ End Frame.
+
+ (** Domain of call stacks *)
+ Module Type CALLSTACK.
+   Definition t : Type := list Frame.t.
+ End CALLSTACK.
+
+ Module CallStack.
+   Definition t : Type := list Frame.t.
+ End CallStack.
+
+ Module Type EXCEPTION_FRAME.
+   Inductive t : Type := 
+      make : Method -> PC -> Location -> LocalVar.t -> t.
+ End EXCEPTION_FRAME.
+ Module ExceptionFrame.
+    Inductive t : Type := 
+      make : Method -> PC -> Location -> LocalVar.t -> t.
+  End ExceptionFrame.
+ 
+ (** Domain of states *)
+ Module Type STATE.
+   Inductive t : Type := 
+      normal : Heap.t -> Frame.t -> CallStack.t -> t
+    | exception : Heap.t -> ExceptionFrame.t -> CallStack.t -> t.
+   Definition get_sf  (s:t) : CallStack.t :=
+     match s with
+       normal _ _ sf => sf
+     | exception _ _ sf => sf
+     end.
+   Definition get_m (s:t) : Method :=
+     match s with
+       normal _ (Frame.make m _ _)_ => m
+     | exception _ (ExceptionFrame.make m _ _ _) _ => m
+     end.
+ End STATE.
+
+ Module State.
+  Inductive t : Type := 
+      normal : Heap.t -> Frame.t -> CallStack.t -> t
+    | exception : Heap.t -> ExceptionFrame.t -> CallStack.t -> t.
+   Definition get_sf (s:t) : CallStack.t :=
+     match s with
+       normal _ _ sf => sf
+     | exception _ _ sf => sf
+     end.
+   Definition get_m (s:t) : Method :=
+     match s with
+       normal _ (Frame.make m _ _)_ => m
+     | exception _ (ExceptionFrame.make m _ _ _) _ => m
+     end.
+ End State.
+ (** Some notations *)
+ Notation St := State.normal.
+ Notation StE := State.exception.
+ Notation Fr := Frame.make.
+ Notation FrE := ExceptionFrame.make.
+
+  (** compatibility between ArrayKind and type *) 
+  Inductive compat_ArrayKind_type : ArrayKind -> type -> Prop :=
+    | compat_ArrayKind_type_ref : forall rt,
+        compat_ArrayKind_type Aarray (ReferenceType rt)
+    | compat_ArrayKind_type_int : 
+        compat_ArrayKind_type Iarray (PrimitiveType INT)
+    | compat_ArrayKind_type_byte : 
+        compat_ArrayKind_type Barray (PrimitiveType BYTE)
+    | compat_ArrayKind_type_bool : 
+        compat_ArrayKind_type Barray (PrimitiveType BOOLEAN)
+    | compat_ArrayKind_type_short : 
+        compat_ArrayKind_type Sarray (PrimitiveType SHORT).
+
+  Inductive isReference : value -> Prop :=
+  | isReference_null : isReference Null
+  | isReference_ref : forall loc, isReference (Ref loc).
+
+  (** compatibility between ValKind and value *) 
+  Inductive compat_ValKind_value : ValKind -> value -> Prop :=
+    | compat_ValKind_value_ref : forall v,
+        isReference v -> compat_ValKind_value Aval v
+    | compat_ValKind_value_int : forall n,
+        compat_ValKind_value Ival (Num (I n)).
+
+  (** compatibility between ArrayKind and value *) 
+  Inductive compat_ArrayKind_value : ArrayKind -> value -> Prop :=
+    | compat_ArrayKind_value_ref : forall v,
+        isReference v -> compat_ArrayKind_value Aarray v
+    | compat_ArrayKind_value_int : forall n,
+        compat_ArrayKind_value Iarray (Num (I n))
+    | compat_ArrayKind_value_byte : forall n,
+        compat_ArrayKind_value Barray (Num (B n))
+    | compat_ArrayKind_value_short : forall n,
+        compat_ArrayKind_value Sarray (Num (Sh n)).
+
+  (* convert a value to be pushed on the stack *)
+  Definition conv_for_stack (v:value) : value :=
+    match v with
+    | Num (B b) => Num (I (b2i b))
+    | Num (Sh s) => Num (I (s2i s))
+    | _ => v
+    end.
+
+  (* convert a value to be store in an array *)
+  Definition conv_for_array (v:value) (t:type) : value :=
+    match v with
+    | Ref loc => v
+    | Num (I i) =>
+       match t with
+         ReferenceType _ => v (* impossible case *)
+       | PrimitiveType INT => v
+       | PrimitiveType BOOLEAN => Num (B (i2bool i))
+       | PrimitiveType BYTE => Num (B (i2b i))
+       | PrimitiveType SHORT => Num (Sh (i2s i))         
+       end
+    | _ => v (* impossible case *)
+    end.
+
+  (** [assign_compatible_num source target] holds if a numeric value [source] can be 
+    assigned to a variable of type [target]. This point is not clear in the JVM spec. *)
+  Inductive assign_compatible_num : num -> primitiveType -> Prop :=
+   | assign_compatible_int_int : forall i, assign_compatible_num (I i) INT
+   | assign_compatible_short_int : forall sh, assign_compatible_num (Sh sh) INT
+   | assign_compatible_byte_int : forall b, assign_compatible_num (B b) INT
+   | assign_compatible_short_short : forall sh, assign_compatible_num (Sh sh) SHORT
+   | assign_compatible_byte_byte : forall b, assign_compatible_num (B b) BYTE
+   | assign_compatible_byte_boolean : forall b, assign_compatible_num (B b) BOOLEAN.
+
+  (** [assign_compatible h source target] holds if a value [source] can be 
+    assigned to a variable of type [target] *)
+  Inductive assign_compatible (p:Program) (h:Heap.t) : value -> type -> Prop :=
+   | assign_compatible_null : forall t, assign_compatible p h Null (ReferenceType t)
+   | assign_compatible_ref_object_val : forall (loc:Location) (t:refType) (cn:ClassName), 
+       Heap.typeof h loc = Some (Heap.LocationObject cn) ->
+       compat_refType p (ClassType cn) t ->
+       assign_compatible p h (Ref loc) (ReferenceType t)
+   | assign_compatible_ref_array_val : forall (loc:Location) (t:refType) (length:Int.t) (tp:type) a, 
+       Heap.typeof h loc = Some (Heap.LocationArray length tp a) ->
+       compat_refType p (ArrayType tp) t ->
+       assign_compatible p h (Ref loc) (ReferenceType t)
+   | assign_compatible_num_val : forall (n:num) (t:primitiveType),
+       assign_compatible_num n t -> assign_compatible p h (Num n) (PrimitiveType t).
+
+  Inductive SemCompRef : CompRef -> value -> value -> Prop :=
+  | SemCompRef_eq : forall v1 v2,
+       isReference v1 -> isReference v2 -> v1 = v2 ->
+     (****************************************************)
+          SemCompRef EqRef v1 v2
+  | SemCompRef_ne : forall v1 v2,
+       isReference v1 -> isReference v2 -> v1 <> v2 ->
+     (****************************************************)
+          SemCompRef NeRef v1 v2.
+
+  Definition SemCompInt (cmp:CompInt) (z1 z2: Z) : Prop :=
+    match cmp with
+      EqInt =>  z1=z2
+    | NeInt => z1<>z2
+    | LtInt => z1<z2
+    | LeInt => z1<=z2
+    | GtInt => z1>z2
+    | GeInt => z1>=z2
+    end.
+
+  Definition SemBinopInt (op:BinopInt) (i1 i2:Int.t) : Int.t :=
+    match op with 
+    | AddInt => Int.add i1 i2
+    | AndInt => Int.and i1 i2
+    | DivInt => Int.div i1 i2
+    | MulInt => Int.mul i1 i2
+    | OrInt => Int.or i1 i2
+    | RemInt => Int.rem i1 i2
+    | ShlInt => Int.shl i1 i2
+    | ShrInt => Int.shr i1 i2
+    | SubInt => Int.sub i1 i2
+    | UshrInt => Int.ushr i1 i2
+    | XorInt => Int.xor i1 i2
+    end.
+(*
+  Inductive CaughtException  (p:Program) : Method -> PC*Heap.t*Location -> PC -> Prop :=
+    CaughtException_def : forall m pc h loc bm pc' e,
+      METHOD.body m = Some bm ->
+      Heap.typeof h loc = Some (Heap.LocationObject e) ->
+      lookup_handlers p (BYTECODEMETHOD.exceptionHandlers bm) pc e pc' ->
+      CaughtException p m (pc,h,loc) pc'.
+
+  Inductive UnCaughtException  (p:Program) : Method -> PC*Heap.t*Location -> Prop :=
+    UnCaughtException_def : forall m pc h loc bm e,
+      METHOD.body m = Some bm ->
+      Heap.typeof h loc = Some (Heap.LocationObject e) ->
+      (forall pc', ~ lookup_handlers p (BYTECODEMETHOD.exceptionHandlers bm) pc e pc') ->
+      UnCaughtException p m (pc,h,loc).
+*)
+End Dom.
+
