ImplemSubClass.v
@@ -1,0 +1,366 @@
+(** * Bicalano: Implementation of a subclass test *)
+
+Require Import List.
+
+Set Implicit Arguments.
+
+Section FOLD.
+
+Variable A : Type.
+Variable f : A -> option A.
+
+Fixpoint fold_opt (l:list A) : option (list A) :=
+  match l with
+  | nil  => None
+  | a::l =>
+    match f a with
+    | None =>
+      match fold_opt l with
+      | None => None
+      | Some l' => Some (a::l')
+      end
+    | Some a' => Some (a' :: l)  
+    end
+  end.
+
+End FOLD.
+
+Section SUBCLASS.
+
+Variable name : Set.
+Variable class : Type.
+Variable get_name : class -> name.
+Variable eq_name : name -> name -> bool.
+Variable superclass : class -> option name.
+
+Inductive tree : Set :=
+  node : name -> list tree -> tree.
+
+Fixpoint get_tree  (n:name) (lt: list tree) {struct lt} : 
+                                    option (tree * list tree) := 
+  match lt with
+  | nil => None
+  | t :: lt => 
+    let (x,_) := t in
+    if eq_name x n then Some (t, lt)
+    else match get_tree n lt with
+    | None => None
+    | Some (nt,lt) => Some (nt, t::lt)
+    end
+  end. 
+
+Definition init_tree n lt :=
+  match get_tree n lt with
+  | None => (node n nil, lt)
+  | Some(tc, lt) => (tc, lt)
+  end.
+    
+Fixpoint add_subclass (s:name) (c:tree) (t:tree) {struct t} : option tree :=
+  match t with
+  | node x l =>
+    if eq_name x s then Some (node x (c::l))
+    else match fold_opt (add_subclass s c) l with
+    | None => None
+    | Some l => Some (node x l)
+    end
+  end.
+  
+Section BUILD_TREE.
+
+ Variable obj : name.
+
+ Fixpoint build_tree (lt:list tree) (l:list class) {struct l} : 
+                                                               list tree :=
+   match l with   
+   | nil => lt
+   | c::l => 
+     let (tc,lt) := init_tree (get_name c) lt in
+     let super := match superclass c with Some s => s | None => obj end in
+     let lt := 
+       match fold_opt (add_subclass super tc) lt with
+       | Some lt => lt
+       | None => (node super (cons tc nil)) :: lt
+       end in
+     build_tree lt l 
+   end.
+  
+End BUILD_TREE.
+
+
+Variable map : Type -> Type.
+Variable empty : forall C:Set, map C.
+Variable update : forall C:Set, map C -> name -> C -> map C.
+Variable get : forall C:Set, map C -> name -> option C.
+
+Fixpoint build_supers (super:list name) (t:tree) (m:map(list name)){struct t} :
+                            map (list name) := 
+  match t with
+  | node a lt =>
+    update (fold_right (build_supers (a::super)) m lt) a super
+  end.
+
+Fixpoint test_In (a:name) (l:list name) {struct l} : bool :=
+  match l with
+    nil => false
+  | x::q => if eq_name a x then true else test_In a q
+  end.
+
+Fixpoint get_obj (l:list class) : option (name * list class) := 
+ match l with
+ | nil => None
+ | c::l =>
+    match superclass c with
+    | None => Some (get_name c, l)
+    | Some _ =>
+      match get_obj l with
+      | None => None
+      | Some (obj, l) => Some (obj, c::l)
+      end
+    end
+ end.
+
+Definition subclass_test (l:list class) : option (name -> name -> bool) :=
+  match get_obj l with
+  | None => None
+  | Some (obj, l) =>
+    match build_tree obj nil l with
+    | t::nil =>
+      let m := build_supers nil t (empty (list name)) in
+      Some (fun x y =>
+              match get m x with
+              | None => false
+              | Some supers => if eq_name x y then true else test_In y supers
+              end)
+    | _ => None
+    end 
+  end.
+
+End SUBCLASS.
+
+
+(*
+
+
+
+
+
+
+
+
+
+
+
+
+
+
+
+
+
+
+
+
+
+
+
+
+
+
+
+
+
+Section __A__.
+Variable A : Set.
+Variable test : A -> A -> bool.
+
+Inductive tree (A:Set) : Set :=
+  node : A -> list (tree A) -> tree A.
+
+Section fold_opt.
+Variable B:Set.
+Variable f:B->option B.
+
+Fixpoint fold_opt (l:list B) {struct l} : option (list B) :=
+ match l with
+   nil => None
+ | a::q =>
+    match f a with
+     | Some a' => Some (a'::q)
+     | None => 
+        match fold_opt q with
+          None => None
+        | Some q' => Some (a::q')
+        end
+    end
+ end.
+
+End fold_opt.
+
+Fixpoint add (n s:A) (t:tree A) {struct t} : option (tree A) :=
+  match t with
+    node x l =>
+      if test x s then Some (node x (node n nil::l))
+      else
+        match fold_opt (add n s) l with
+          None => None
+        | Some l' => Some (node x  l')
+        end
+  end.
+
+Variable class : Set.
+Variable name : class -> A.
+Variable superclass : class -> option A.
+
+Fixpoint build_tree_rec (t:tree A) (l:list class) {struct l} : option (tree A) :=
+ match l with
+  nil => Some t
+ | c::q => 
+     match superclass c with
+      Some s =>
+         match (add (name c) s t) with
+          None => None
+        | Some t' => build_tree_rec t' q
+        end
+     | _ => None
+     end
+ end.
+
+Definition build_tree (l:list class) : option (tree A) :=
+ match l with 
+ | nil => None
+ | c::l => 
+    match superclass c with
+     None => build_tree_rec (node (name c) nil) l
+    | _ => None
+    end
+ end.
+
+Fixpoint test_In (a:A) (l:list A) {struct l} : bool :=
+  match l with
+    nil => false
+  | x::q => if test a x then true else test_In a q
+  end.
+
+Fixpoint find (C:Set) (a:A) (l:list (A*C)) {struct l} : option C :=
+  match l with
+    nil => None
+  | (x,c)::q => if test a x then Some c else find a q
+  end.
+
+Variable B:Set -> Set.
+Variable empty : forall C:Set, B C.
+Variable update : forall C:Set, B C -> A -> C -> B C.
+Variable get : forall C:Set, B C -> A -> option C.
+
+Fixpoint build_supers (l:list A) (t:tree A) (b:B (list A)) {struct t}  : B (list A) := 
+  match t with
+    node a ltt =>
+      update (fold_right (build_supers (a::l)) b ltt)  a l
+  end.
+
+Definition subclass_test (l:list class) : option (A -> A -> bool) :=
+  match build_tree l with
+    None => None
+  | Some t =>
+      let m := build_supers nil t (empty (list A)) in
+        Some (fun x y =>
+                match get m x with
+                  None => false
+                | Some supers => test_In y supers
+                end)
+  end.
+
+End __A__.
+
+
+
+
+
+
+
+
+
+
+
+
+
+
+
+
+
+
+
+
+
+
+(*
+
+Definition l : list (class nat) := 
+ (mc 0 None)::(mc 1 (Some 0))::(mc 2 (Some 0))::(mc 3 (Some 0))::
+ (mc 4 (Some 1))::
+ (mc 5 (Some 1))::
+ (mc 6 (Some 4))::
+ (mc 7 (Some 2))::
+ (mc 8 (Some 2))::nil.
+
+Fixpoint nat_eq (n1 n2:nat) {struct n1} : bool :=
+  match n1,n2 with
+    O,O => true
+  | S p1,S p2 => nat_eq p1 p2
+  | _,_ => false
+  end.
+
+Eval compute in build_tree nat_eq l.
+
+Definition t :=
+   (node 0
+      (node 3 nil::
+       node 2 (node 8 nil ::
+               node 7 nil :: nil) ::
+       node 1 (node 5 nil :: 
+               node 4 (node 6 nil :: nil) :: 
+               nil) ::
+       nil)).
+
+
+Definition subclass_nat_test :=
+ @subclass_test nat nat_eq
+   (fun C => list (nat*C))
+   (fun C => @nil (nat*C))
+   (fun C a c b =>cons (a,c) b)
+   (find nat_eq).
+
+Eval compute in
+ @build_supers nat
+      (fun C => list (nat*C))
+   (fun C a c b =>cons (a,c) b)
+   nil t nil.
+
+Definition test (A:Set) (f_op:option (A->A->bool)) :=
+  match f_op with 
+   None => fun _ _ => false
+ | Some f => f
+  end.
+
+Eval compute in test (subclass_nat_test l) 3 0.
+Eval compute in test (subclass_nat_test l) 2 0.
+Eval compute in test (subclass_nat_test l) 8 0.
+Eval compute in test (subclass_nat_test l) 8 2.
+Eval compute in test (subclass_nat_test l) 7 0.
+Eval compute in test (subclass_nat_test l) 7 2.
+Eval compute in test (subclass_nat_test l) 1 0.
+Eval compute in test (subclass_nat_test l) 5 0.
+Eval compute in test (subclass_nat_test l) 5 1.
+Eval compute in test (subclass_nat_test l) 4 0.
+Eval compute in test (subclass_nat_test l) 4 1.
+Eval compute in test (subclass_nat_test l) 6 0.
+Eval compute in test (subclass_nat_test l) 6 1.
+Eval compute in test (subclass_nat_test l) 6 4.
+Eval compute in test (subclass_nat_test l) 6 2.
+Eval compute in test (subclass_nat_test l) 6 3.
+Eval compute in test (subclass_nat_test l) 6 5.
+Eval compute in test (subclass_nat_test l) 6 7.
+Eval compute in test (subclass_nat_test l) 6 8.
+
+
+*)
+*)
